Ajout de balisage

src/CoqNom/examples/example2.v
@@ -15,37 +15,65 @@ Definition octet := N.
 
 Definition data := list octet.
 
+(* =DecodeurM= *)
 Definition DecodeurM (X : Type) := data -> span -> option (X * span).
+(* =end= *)
 
 Equations length (l: data) : N :=
   length nil := 0;
   length (_ :: t) := N.succ (length t).
 
-Definition decodeM {X} (d : DecodeurM X) (l : data) : option X :=
+Section decodeM.
+
+  Context {X : Type}.
+
+(* =decodeM= *)
+Definition decodeM (d : DecodeurM X) (l : data) : option X :=
   match d l (mk_span 0 (length l)) with
   | None => None
   | Some (v, _) => Some v
   end.
+(* =end= *)
 
-Definition pure {X} (v : X) : DecodeurM X := fun data l => Some (v,l).
+End decodeM.
 
-Definition bind {X Y} (d : DecodeurM X) (k : X -> DecodeurM Y) : DecodeurM Y :=
+Section pure.
+
+  Context {X : Type}.
+(* =pure= *)
+Definition pure (v : X) : DecodeurM X := fun data l => Some (v,l).
+(* =end= *)
+
+End pure.
+
+Section bind.
+
+  Context {X Y : Type}.
+
+(* =bind= *)
+Definition bind (d : DecodeurM X) (k : X -> DecodeurM Y) : DecodeurM Y :=
   fun data l =>
     match d data l with
     | None => None
     | Some (v, s) => k v data s
     end.
+(* =end= *)
+
+End bind.
 
 Notation "'let!' v ':=' f 'in' g" := (bind f (fun v => g)) (v name, at level 50).
 Notation "'ret!' v" := (pure v) (at level 50).
 
+(* =app= *)
 Definition app {X Y} (a : DecodeurM (X -> Y)) (d : DecodeurM X) : DecodeurM Y :=
   let! f := a in
   let! x := d in
   ret! (f x).
+(* =end= *)
 
 Notation " f '<*>' g" := (app f g)(at level 50).
 
+(* =takeM= *)
 Definition takeM (n : N) : DecodeurM span :=
   fun _ s =>
     if n <=? len s
@@ -55,6 +83,7 @@ Definition takeM (n : N) : DecodeurM span :=
       Some (res, sres)
     else
       None.
+(* =end= *)
 
 Equations lookup (n : N) (l : data) : option N by wf (N.to_nat n) Nat.lt :=
   lookup n [] := None;
@@ -64,6 +93,7 @@ Next Obligation.
   lia.
 Defined.
 
+(* =readM= *)
 Definition readM (s : span) (n : N) : DecodeurM N :=
   fun d t =>
     if n <? len s
@@ -74,22 +104,35 @@ Definition readM (s : span) (n : N) : DecodeurM N :=
       end
     else
       None.
+(* =end= *)
 
-Definition decode_nextM : DecodeurM N :=
+(* =decode_next= *)
+Definition decode_next : DecodeurM N :=
   let! s := takeM 1 in
   readM s 0.
+(* =end= *)
 
+(* =failM= *)
 Definition failM {X} : DecodeurM X := fun _ _ => None.
+(* =end= *)
 
 Definition to_u32 (a0 a1 a2 a3 : octet) : N :=
   a0 * (N.pow 2 32) + a1 * (N.pow 2 16) + a2  * (N.pow 2 8) + a3.
 
+(* =decode_packet_length= *)
 Definition decode_packet_length : DecodeurM N :=
-  pure to_u32 <*> decode_nextM <*> decode_nextM <*> decode_nextM <*> decode_nextM.
+  pure to_u32 <*> decode_next <*> decode_next <*> decode_next <*> decode_next.
+(* =end= *)
 
+(* =decode_payload_SSH= *)
 Definition decode_payload_SSH : DecodeurM span :=
   let! packet_length := decode_packet_length in
-  let! padding_length := decode_nextM in
-  let! payload := takeM (packet_length - padding_length - 1) in
-  let! padding := takeM padding_length in
-  ret! payload.
+  let! padding_length := decode_next in
+  if padding_length + 1 <=? packet_length
+  then
+    let! payload := takeM (packet_length - padding_length - 1) in
+    let! padding := takeM padding_length in
+    ret! payload
+  else
+    failM.
+(* =end= *)
